
\begin{problem}
  \emph{Recall that $\Sigma ; \alpha = \Sigma \cup \{ \alpha \}$,
  the set $\Sigma$ together with the one possibly new member $\alpha$.}
  \\
  Show that the following hold:
  \begin{enumalph}
    \item $\Sigma ; \alpha \models \beta \iff \Sigma \models (\alpha \lto \beta)$.
    \begin{Answer}
      \begin{enumroman}
        \item $\Sigma ; \alpha \models \beta \implies \Sigma \models (\alpha \lto \beta)$
        
          \step
          Suppose $\Sigma ; \alpha \models \beta$.
          Let $v$ be a truth assignment satisfying $\Sigma$.

          \step
          If $\vbar(\alpha) = T$, then $v$ satisfies $\Sigma ; \alpha$
          (since $v$ already satisfies $\Sigma$), and $\Sigma ; \alpha \models \beta$,
          implying that $\vbar(\beta) = T$.
          Therefore, $\vbar(\alpha \lto \beta) = (T \lto T) = T$.

          \step
          If $\vbar(\alpha) = F$, then $\vbar(\alpha \lto \beta) = (F \lto \vbar(\beta)) = T$.

        \step
        \item $\Sigma ; \alpha \models \beta \backimplies \Sigma \models (\alpha \lto \beta)$
        
          \step
          Suppose $\Sigma \models (\alpha \lto \beta)$ but $\Sigma ; \alpha \nmodels \beta$.

          \step
          Let $v$ be a truth assignment satisfying $\Sigma$.
          Suppose $\vbar(\alpha) = T$.
          \begin{itemize}
            \item First, we can note that
              $\vbar(\alpha) = T$ implies that $v$ satisfies $\Sigma ; \alpha$,
              which further implies that $\vbar(\beta) = F$, since $\Sigma ; \alpha \nmodels \beta$.
            \item Next, since $\Sigma \models (\alpha \to \beta)$,
              $\vbar(\alpha) = T$ implies $\vbar(\beta) = T$. This is a contradiction.
          \end{itemize}
        Therefore, it must be the case that $\Sigma \models (\alpha \lto \beta) \implies \Sigma ; \alpha \models \beta $
      \end{enumroman}
    \end{Answer}
    \item $\alpha \models \backmodels \beta \iff \models (\alpha \leftrightarrow \beta)$.  
    \begin{Answer}
      Let $v$ be any truth assignment to $\alpha$ and $\beta$
      satisfying the wff $\alpha \models \backmodels \beta$. Then:
      \begin{itemize}
        \item $\vbar(\beta) = T$ whenever $\vbar(\alpha) = T$ (since $\alpha \models \beta)$.
        \item $\vbar(\alpha) = T$ whenever $\vbar(\beta) = T$ (since $\beta \models \alpha)$.
        \item Consequently, $\lnot (\vbar(\alpha)) \leftrightarrow \lnot (\vbar(\beta))$,
        implying that $\vbar(\alpha \leftrightarrow \beta) = T$.
      \end{itemize}
      Therefore, any truth assignment to $\alpha$ and $\beta$
      satisfying the wff $\alpha \models \backmodels \beta$ also satisfies
      $\models (\alpha \leftrightarrow \beta)$.
    \end{Answer}
  \end{enumalph}
\end{problem}
