

\crefformat{cor}{format}
\begin{problem}
  Prove or refute each of the following assertions:
  \begin{enumalph}
    \item If either $\Sigma \models \alpha$ or $\Sigma \models \beta$,
      then $\Sigma \models (\alpha \lor \beta)$.
      \begin{Answer}
        True.
        
        \step
        Suppose $\Sigma \models \alpha$, and let $v$ be any truth assignment satisfying $\Sigma$.
        Then $\vbar(\alpha) = T$, which implies that $\vbar(\alpha \lor \beta)
        = (T \lor \vbar(\beta)) = T$.

        \noindent
        Therefore, $\Sigma \models \alpha \implies \Sigma \models (\alpha \lor \beta)$.

        \step
        In the alternate case, suppose $\Sigma \models \beta$,
        and let $v$ be a truth assignment satisfying $\Sigma$.
        Then $\vbar(\beta)~=~T$, which implies that $\vbar(\alpha \lor \beta)
        = (\vbar(\alpha) \lor T) = T$.

        \noindent
        Therefore, $\Sigma \models \beta \implies \Sigma \models (\alpha \lor \beta)$.
      \end{Answer}
    \item If $\Sigma \models (\alpha \lor \beta)$, then either $\Sigma \models \alpha$
      or $\Sigma \models \beta$.
      \begin{Answer}
        True.

        \step
        Suppose $\Sigma \models (\alpha \lor \beta)$ but $\Sigma \nmodels \alpha$ and $\Sigma \nmodels \beta$.

        \noindent
        Let $v$ be any truth assignment satisfying $\Sigma$, then:
        \begin{itemize}
          \item $\vbar(\alpha \lor \beta) = T$ since $\Sigma \models (\alpha \lor \beta)$,
            which implies that either $\vbar(\alpha) = T$ or $\vbar(\beta) = T$.
          \item $\vbar(\alpha) = F$ since $\Sigma \nmodels \alpha$.
          \item $\vbar(\beta) = F$ since $\Sigma \nmodels \beta$.
        \end{itemize}
        This is a clear contradiction, thus it must be the case that either
        $\Sigma \models \alpha$ or $\Sigma \models \beta$ whenever $\Sigma \models (\alpha \lor \beta)$.
      \end{Answer}
  \end{enumalph}
\end{problem}

