\begin{problem}[1]
  \begin{enumalph}
    \item Show that $\Gamma ; \alpha \models \phi$ iff $\Gamma \models (\alpha \to \phi)$.
  \end{enumalph}
\end{problem}
\begin{Answer}
  
  \step
  Let $\fA$ be a model for $\Gamma$ and let $s : V \to \abs{\fA}$
  be a function such that $\fA$ satisfies $\Gamma$ with $s$.
  Then $\models_{\fA} \gamma[s]$ for all $\gamma \in \Gamma$.
  Then:

  \step
  ($\Rightarrow$)
  We shall prove the right implication via the contrapositive,
  i.e. if $\Gamma \not \models (\alpha \to \phi)$
  then $\Gamma ; \alpha \not \models \phi$.

  \step
  Suppose $\Gamma \not \models (\alpha \to \phi)$.
  Since $\fA$ satisfies $\Gamma$ with $s$
  and $\Gamma \not \models (\alpha \to \phi)$,
  it must be the case that $\sbar(\alpha) = T$ and $\sbar(\phi) = F$
  so that $\sbar(\alpha \to \phi) = F$.
  Therefore, $\fA$ satisfies $\Gamma ; \alpha$ with $s$,
  but since $\fA$ does not satisfy $\phi$ with $s$,
  it must be the case that $\Gamma ; \alpha \not \models \phi$.
  
  \bigskip
  \bigskip
  \step
    ($\Leftarrow$)
    We shall prove this directly, i.e. by showing that
    if $\Gamma \models (\alpha \to \phi)$ then
    $\Gamma ; \alpha \models \phi$.

    \step
    Suppose $\Gamma \models (\alpha \to \phi)$,
    we show that it is always the case that $\Gamma ; \alpha \models \phi$.
    \begin{enumroman}
      \item If $\fA$ does not satisfy $\alpha$ with $s$, then
        $\not \models_{\fA} \alpha[s]$. Therefore,
        $\sbar(\alpha) = F$, so $\sbar(\alpha \to \phi) = T$
        irrespective of the value of $\sbar(\phi)$,
        so $\models_{\fA} (\alpha \to \phi)[s]$.
        Since $\sbar(\alpha) = F$ and $a \to \phi$,
        $\Gamma ; \alpha \models \phi$.
      \item If $\fA$ satisfies $\alpha$ with $s$, then
        $\models_{\fA} \alpha[s]$, so $\sbar(\alpha) = T$.
        Therefore, $\sbar(\alpha \to \phi) = \sbar(\phi)$.
        Since $\Gamma \models (\alpha \to \phi)$,
        and $\fA$ satisfies $\Gamma$ with $s$,
        then $\fA$ satisfies $\phi$ with $s$.
        so $\models_{\fA} (\alpha \to \phi)[s]$.
        Since $\sbar(\alpha) = T$ and $\sbar(\phi) = T$,
        $\Gamma ; \alpha \models \phi$.
    \end{enumroman}
\end{Answer}
